Uppaal_Networks/AbsInt/AbsInt_Refine.thy
@@ -78,7 +78,7 @@ lemma single_lookup_le: "x \<le> single k v \<Longrightarrow> lookup x k \<le> v
 lemma r_single_structure: "\<exists>m. r_single k v = Mapping m"
   by (metis bot_mapping_def empty_Mapping insert_Mapping r_single.simps)
 
-fun merge_single :: "('a::bounded_semilattice_sup_bot) state_map \<Rightarrow> addr \<Rightarrow> 'a \<Rightarrow> 'a state_map" where
+fun merge_single :: "('a::{semilattice_sup , order_bot}) state_map \<Rightarrow> addr \<Rightarrow> 'a \<Rightarrow> 'a state_map" where
   "merge_single (SM m) pc x = SM (\<lambda>npc. if npc = pc then x \<squnion> m npc else m npc)"
 
 lemma merge_single_grows: "m \<le> merge_single m pc x"
@@ -92,10 +92,10 @@ lemma merge_single_bot: "merge_single a k \<bottom> = a"
 proof (rule state_map_eq_fwd)
   fix p
   obtain m where "a = SM m" using state_map_single_constructor by blast
-  then show "lookup (merge_single a k \<bottom>) p = lookup a p" by simp
+  then show "lookup (merge_single a k \<bottom>) p = lookup a p" by (simp add: sup.absorb2)
 qed
 
-fun r_merge_single :: "('a::{bounded_semilattice_sup_bot}) r_state_map \<Rightarrow> addr \<Rightarrow> 'a \<Rightarrow> 'a r_state_map" where
+fun r_merge_single :: "('a::{semilattice_sup, order_bot}) r_state_map \<Rightarrow> addr \<Rightarrow> 'a \<Rightarrow> 'a r_state_map" where
   "r_merge_single tree pc x = Mapping.update pc (x \<squnion> (r_lookup tree pc)) tree"
 
 lemma merge_single_neq:
@@ -218,7 +218,7 @@ qed
 lemma sup_mapping_aux_structure: "\<exists>m. sup_mapping_aux b pc (Mapping acc) = Mapping m"
   using insert_Mapping by fastforce
 
-instantiation mapping :: (linorder, "bounded_semilattice_sup_bot") sup
+instantiation mapping :: (linorder, "{semilattice_sup, order_bot}") sup
 begin
 fun sup_mapping :: "('a, 'b) mapping \<Rightarrow> ('a, 'b) mapping \<Rightarrow> ('a, 'b) mapping" where
   "sup_mapping a b = fold
@@ -240,7 +240,7 @@ text \<open>
 It's not possible to instantiate mapping :: order
 but we can still have some lemmas from semilattice_sup outside instantiations:
 \<close>
-lemma mapping_sup_ge1 [simp]: "(x::('a::linorder, 'b::bounded_semilattice_sup_bot) mapping) \<le> x \<squnion> y"
+lemma mapping_sup_ge1 [simp]: "(x::('a::linorder, 'b::{semilattice_sup, order_bot}) mapping) \<le> x \<squnion> y"
 proof -
   have "acc \<le> (sup_mapping_aux y) a acc" for a acc using sup_mapping_aux_grows by simp
   thus ?thesis by (simp add: fold_grow)
@@ -266,7 +266,7 @@ using assms proof(induction "sorted_list_of_set (r_domain b)" arbitrary: a b)
     assume "\<not> r_lookup b pc = \<bottom>"
     thus False using r_domain nob by fastforce
   qed
-  then show ?case using left by simp
+  then show ?case using left by (simp add: sup.absorb1)
 next
   case (Cons x xs)
 
@@ -295,12 +295,12 @@ next
 
   from xs_bprev finite_bprev have lookup_prev: "r_lookup (?anext \<squnion> ?bprev) pc = r_lookup ?anext pc \<squnion> r_lookup ?bprev pc" by (rule Cons(1))
   from foldbprev_concrete this show ?case
-    by (metis (mono_tags, lifting) lookup_default_update lookup_default_update_neq r_lookup.simps sup_bot.right_neutral sup_mapping.simps sup_mapping_aux.elims xs_bprev)
+    by (metis (no_types, lifting) bot.extremum lookup_default_update lookup_default_update_neq r_lookup.simps sup.orderE sup_mapping.simps sup_mapping_aux.elims xs_bprev)
 qed
 
 lemma mapping_sup_ge2:
   assumes "finite (r_domain y)"
-  shows "(y::('a::linorder, 'b::bounded_semilattice_sup_bot) mapping) \<le> x \<squnion> y"
+  shows "(y::('a::linorder, 'b::{semilattice_sup, order_bot}) mapping) \<le> x \<squnion> y"
 proof(rule mapping_leI)
   fix p
   from assms have "r_lookup (x \<squnion> y) p = r_lookup x p \<squnion> r_lookup y p" by (rule mapping_sup_lookup)
@@ -309,7 +309,7 @@ qed
 
 lemma mapping_sup_least:
   assumes
-    "(y::('a::linorder, 'b::bounded_semilattice_sup_bot) mapping) \<le> x"
+    "(y::('a::linorder, 'b::{semilattice_sup, order_bot}) mapping) \<le> x"
     "z \<le> x"
   shows "y \<squnion> z \<le> x"
 proof(rule mapping_leI)
@@ -318,7 +318,7 @@ proof(rule mapping_leI)
     by (metis List.fold_simps(1) le_sup_iff less_eq_mapping_def mapping_sup_lookup sorted_list_of_set.infinite sup_mapping.simps)
 qed
 
-lemma mapping_sup[code]: "((RSM a)::'a::bounded_semilattice_sup_bot state_map) \<squnion> RSM (Mapping bm) = RSM (a \<squnion> (Mapping bm))"
+lemma mapping_sup[code]: "((RSM a)::'a::{semilattice_sup, order_bot} state_map) \<squnion> RSM (Mapping bm) = RSM (a \<squnion> (Mapping bm))"
 proof (rule state_map_eq_fwd)
   let ?b = "Mapping bm"
   have "finite (r_domain ?b)" using r_domain_finite by blast
@@ -540,7 +540,8 @@ proof(rule state_map_eq_fwd)
           "?l = pre @ ipc # post"
           "lookup (fold ?f pre \<bottom>) pc \<le> y"
           "\<not> lookup (?f ipc (fold ?f pre \<bottom>)) pc \<le> y"
-          using fold_overgrowth_lookup by (metis bot_lookup r_step_map_from_grows sup.orderI sup_bot.right_neutral)
+          using fold_overgrowth_lookup
+          by (metis bot.extremum r_step_map_from_grows single_lookup_le)
         let ?prefold = "fold ?f pre \<bottom>"
 
         have "\<exists>op. Some op = prog ipc" proof (cases "prog ipc")
@@ -656,7 +657,7 @@ lemma deep_merge_init: "deep_merge (set s) \<squnion> (RSM (Mapping init)) = RSM
 proof(induction s arbitrary: init)
   case Nil
   let ?init = "Mapping init"
-  have l: "deep_merge (set []) \<squnion> (RSM ?init) = RSM ?init" by (metis deep_merge_empty list.set(1) sup_bot.left_neutral)
+  have l: "deep_merge (set []) \<squnion> (RSM ?init) = RSM ?init" by (metis bot.extremum deep_merge_empty list.set(1) sup.absorb2)
   have r: "r_deep_merge_l [] ?init = ?init" by (simp add: bot_mapping_def lookup_default_empty)
   from l r show ?case by simp
 next
@@ -682,7 +683,7 @@ next
     case True
     hence lreduce: "deep_merge (set (x # xs)) = deep_merge (set xs)" using deep_merge_bot using x by blast
     have "RSM (r_deep_merge_l (x # xs) (RBT_Mapping.Mapping init)) = RSM (r_deep_merge_l xs \<bottom>) \<squnion> RSM (RBT_Mapping.Mapping init)" using r_deep_merge_l_bot
-      by (metis Cons.IH True boolean_algebra_cancel.sup0 bot_mapping_def empty_Mapping r_bot r_empty_map_def x)
+      by (metis Cons.IH True bot.extremum bot_mapping_def empty_Mapping r_bot r_empty_map_def sup.absorb2 sup_commute x)
     from this lreduce show ?thesis by (metis Cons.IH True r_deep_merge_l_bot x)
   next
     case False
@@ -698,7 +699,7 @@ proof -
   have "deep_merge (set s) \<squnion> (RSM (Mapping init)) = RSM (r_deep_merge_l s (Mapping init))" by (rule deep_merge_init)
   from this init have "deep_merge (set s) \<squnion> (RSM \<bottom>) = RSM (r_deep_merge_l s \<bottom>)" by simp
   hence "deep_merge (set s) \<squnion> \<bottom> = RSM (r_deep_merge_l s \<bottom>)" by (simp add: r_bot bot_mapping_def r_empty_map_def)
-  thus ?thesis by simp
+  thus ?thesis by (simp add: sup.absorb1)
 qed
 
 fun list_is_singleton :: "'a list \<Rightarrow> bool" where
