Uppaal_Networks/AbsInt/OptionLattice.thy
@@ -1,76 +1,7 @@
 theory OptionLattice
-imports AbsInt Word PowerBool
+imports AbsInt Abs_Word PowerBool
+  "HOL-Library.Option_ord"
 begin
-
-instantiation option :: (order) order begin
-  fun less_eq_option :: "('a::order) option \<Rightarrow> 'a option \<Rightarrow> bool" where
-    "less_eq_option None _ \<longleftrightarrow> True" |
-    "less_eq_option (Some x) None \<longleftrightarrow> False" |
-    "less_eq_option (Some x) (Some y) \<longleftrightarrow> x \<le> y"
-
-  fun less_option :: "'a option \<Rightarrow> 'a option \<Rightarrow> bool" where
-    "less_option None None \<longleftrightarrow> False" |
-    "less_option None (Some x) \<longleftrightarrow> True" |
-    "less_option (Some x) None \<longleftrightarrow> False" |
-    "less_option (Some x) (Some y) \<longleftrightarrow> x < y"
-instance proof
-  show "((x::'a option) < y) = (x \<le> y \<and> \<not> y \<le> x)" for x y by (cases x; cases y) auto
-  show "(x::'a option) \<le> x" for x by (cases x) auto
-  show "(x::'a option) \<le> z" if "x \<le> y" and "y \<le> z" for x y z
-    using that by (cases x; cases y; cases z) auto
-  show "(x::'a option) = y" if "x \<le> y" and "y \<le> x"for x y
-    using that by (cases x; cases y) auto
-qed
-end
-
-instantiation option :: (type) bot
-begin
-definition[simp]: "\<bottom> \<equiv> None"
-instance ..
-end
-
-instantiation option :: (top) top
-begin
-definition[simp]: "\<top> \<equiv> Some \<top>"
-instance ..
-end
-
-instantiation option :: (sup) sup
-begin
-fun sup_option :: "'a option \<Rightarrow> 'a option \<Rightarrow> 'a option" where
-  "sup_option None b = b" |
-  "sup_option a None = a" |
-  "sup_option (Some a) (Some b) = Some (a \<squnion> b)"
-instance ..
-end
-
-instantiation option :: (inf) inf
-begin
-fun inf_option :: "'a option \<Rightarrow> 'a option \<Rightarrow> 'a option" where
-  "inf_option None _ = None" |
-  "inf_option _ None = None" |
-  "inf_option (Some a) (Some b) = Some (a \<sqinter> b)"
-instance ..
-end
-
-instantiation option :: ("{semilattice_sup, order_top}") bounded_semilattice_sup_bot
-begin
-instance proof (standard, goal_cases)
-  case (1 x y) then show ?case by (cases x; cases y; simp)
-next
-  case (2 y x) then show ?case by (cases x; cases y; simp)
-next
-  case (3 y x z) then show ?case by (cases x; cases y; cases z; simp)
-qed simp
-end
-
-instantiation option :: ("{semilattice_sup, order_top}") order_top
-begin
-instance proof (standard, goal_cases)
-  case (1 a)
-  then show ?case by (cases a; simp)
-qed
-end
 
 instantiation option :: ("{semilattice_sup, order_top}") absstate begin instance .. end
 instantiation option :: ("{semilattice_sup, order_top}") absword begin instance .. end
@@ -191,6 +122,7 @@ proof (cases a)
       have "\<And>f. \<gamma>_option f b = (f bb::'b set)" by (simp add: \<open>b = Some bb\<close>)
       moreover have "\<And>f. \<gamma>_option f a = (f aa::'b set)" by (simp add: Some)
       moreover have "\<And>f. option_le f a b = f aa bb" using Some \<open>b = Some bb\<close> by force
+      moreover have "\<And>f. option_eq f a b = option_le f a b" by (simp add: Some \<open>b = Some bb\<close>)
       ultimately show ?thesis using assms by presburger
     qed
   qed simp
